Add progress on locked queue

DataflowRewriter/LockedQueue.lean
@@ -1,4 +1,5 @@
 import DataflowRewriter.StateTransition
+import Mathlib.Tactic
 
 namespace DataflowRewriter
 
@@ -51,19 +52,37 @@ instance SpecStateTransition : StateTransition Method SpecState where
   init := default
   step := spec_step
 
-section
+infix:60 " ≺ " => @indistinguishable Method
 
-variable {ImpState SpecState : Type}
-
-variable [imp : StateTransition Method ImpState]
-variable [spec : StateTransition Method SpecState]
-
-def indistinguishable (i: ImpState) (s: SpecState): Prop :=
-  ∀ (e: List Method) i', i -[e]-> i' → ∃ s', s -[e]-> s'
-
-infix:60 " ≺ " => indistinguishable
-
-end
+inductive φ' : ImpState → SpecState → Prop where
+  | base :
+    φ' ⟨false, []⟩ ⟨[]⟩
+  | enq : ∀ i (i' : Nat → ImpState) s (s' : Nat → SpecState),
+    (∀ n, i' n = { i with queue := i.queue ++ [n] }) →
+    (∀ n, s' n = { s with queue := s.queue ++ [n] }) →
+    (∀ n, φ' (i' n) (s' n)) →
+    (∀ n, imp_step i [Method.enq n] (i' n)) →
+    (∀ n, spec_step s [Method.enq n] (s' n)) →
+    φ' i s
+  | deq : ∀ i i' s s',
+    φ' i' s' →
+    imp_step i [Method.deq n] i' →
+    spec_step s [Method.deq n] s' →
+    φ' i s
+  | unlock : ∀ i i' s s',
+    φ' i' s' →
+    imp_step i [Method.unlock] i' →
+    spec_step s [Method.unlock] s' →
+    φ' i s
+  | lock : ∀ i i' s s',
+    φ' i' s' →
+    imp_step i [Method.lock] i' →
+    spec_step s [Method.lock] s' →
+    φ' i s
+  | internal : ∀ i i' s,
+    φ' i' s →
+    imp_step i [] i' →
+    φ' i s
 
 inductive φ : ImpState → SpecState → Prop where
   | base :
@@ -71,35 +90,71 @@ inductive φ : ImpState → SpecState → Prop where
   | enq : ∀ i (i' : Nat → ImpState) s (s' : Nat → SpecState),
     (∀ n, i' n = { i with queue := i.queue ++ [n] }) →
     (∀ n, s' n = { s with queue := s.queue ++ [n] }) →
+    i ≺ s → 
     (∀ n, φ (i' n) (s' n)) →
     (∀ n, imp_step i [Method.enq n] (i' n)) →
     (∀ n, spec_step s [Method.enq n] (s' n)) →
     φ i s
-  | deq : ∀ i i' s s',
+  | deq : ∀ i i' s s' n,
+    i ≺ s →
     φ i' s' →
     imp_step i [Method.deq n] i' →
     spec_step s [Method.deq n] s' →
     φ i s
   | unlock : ∀ i i' s s',
+    i ≺ s →
     φ i' s' →
     imp_step i [Method.unlock] i' →
     spec_step s [Method.unlock] s' →
     φ i s
   | lock : ∀ i i' s s',
+    i ≺ s →
     φ i' s' →
     imp_step i [Method.lock] i' →
     spec_step s [Method.lock] s' →
     φ i s
   | internal : ∀ i i' s,
+    i ≺ s →
     φ i' s →
     imp_step i [] i' →
     φ i s
 
+theorem empty_indistinguishable :
+  (default : ImpState) ≺ (default : SpecState) := by
+  unfold indistinguishable; intros e i' Himp
+  cases Himp with
+  | handle_enq n a | handle_lock | handle_unlock => constructor; apply star.plus_one; constructor
+  | handle_deq n rst a => simp at a
+  | unlock_natural => constructor; apply star.refl
+
+theorem φ_indistinguishable i s :
+  φ i s → i ≺ s := by
+  intros H; induction H with
+  | base => apply empty_indistinguishable
+  | _ => assumption
+
+theorem φ_length i s :
+  φ i s → i.queue.length = s.queue.length := by
+  intros H; induction H with
+  | base => simp
+  | enq i i_ne s s_ne i_wf s_wf _ _ _ _ Hlist =>
+    specialize Hlist 0
+    specialize i_wf 0
+    specialize s_wf 0
+    rw [i_wf,s_wf] at Hlist
+    simp at Hlist; assumption
+  | deq i i' s s' n _ Hphi Himp Hspec Hlist
+  | unlock i i' s s' _ Hphi Himp Hspec Hlist
+  | lock i i' s s' _ Hphi Himp Hspec Hlist =>
+    cases Himp; cases Hspec; simp [*]
+  | internal i i' s _ Hphi Himp Hlist =>
+    cases Himp; assumption
+
 theorem enough :
-  ∀ i s, φ i s → 
+  ∀ i s, φ i s →
     ∀ e i', imp_step i e i' → 
       ∃ s', star s e s' ∧ φ i' s' := by
-  intros i s h; 
+  intros i s h;
   induction h with
   | base =>
     intros e i' Himp
@@ -111,6 +166,22 @@ theorem enough :
         · apply φ.base
         · constructor; simp; rfl
         · constructor; simp
+      · unfold indistinguishable at *
+        intros e i' Histep
+        cases Histep with
+        | handle_enq n' a' =>
+          simp at *
+          constructor; apply star.plus_one
+          constructor
+        | handle_deq n' rst' a' =>
+          simp at *
+          rcases a' with ⟨ Hl, Hr ⟩
+          constructor; apply star.plus_one
+          constructor; simp
+          and_intros <;> [congr; rfl]
+        | handle_lock | handle_unlock =>
+          constructor; apply star.plus_one; constructor
+        | unlock_natural => constructor; apply star.refl
     | handle_deq n rst a => simp at a
     | handle_lock =>
       simp; exists ⟨[]⟩; and_intros
@@ -118,22 +189,60 @@ theorem enough :
       · apply φ.unlock; apply φ.base
         · constructor
         · constructor
+      · unfold indistinguishable at *
+        intros e i' Histep
+        cases Histep with
+        | handle_enq n' a' => simp at *
+        | handle_deq n' rst' a' => simp at *
+        | handle_lock | handle_unlock =>
+          constructor; apply star.plus_one; constructor
+        | unlock_natural => constructor; apply star.refl
     | handle_unlock =>
       simp; exists ⟨[]⟩; and_intros
       · apply star.plus_one; constructor
       · apply φ.base
+      · unfold indistinguishable at *
+        intros e i' Histep
+        cases Histep with
+        | handle_enq n' a' =>
+          simp at *
+          constructor; apply star.plus_one
+          constructor
+        | handle_deq n' rst' a' => simp at *
+        | handle_lock | handle_unlock =>
+          constructor; apply star.plus_one; constructor
+        | unlock_natural => constructor; apply star.refl
     | unlock_natural a =>
       simp; exists ⟨[]⟩; and_intros
       · apply star.refl
       · apply φ.base
+      · unfold indistinguishable at *
+        intros e i' Histep
+        cases Histep with
+        | handle_enq n' a' =>
+          simp at *
+          constructor; apply star.plus_one
+          constructor
+        | handle_deq n' rst' a' => simp at *
+        | handle_lock | handle_unlock =>
+          constructor; apply star.plus_one; constructor
+        | unlock_natural => constructor; apply star.refl
   | enq i i_ne s s_ne i_wf s_wf Hphi HimpRight HspecRight iH =>
     intros e i_sw HimpDown
     have HimpDown' := HimpDown
     cases HimpDown with
     | handle_enq n' Hlock =>
-      exists { s with queue := s.queue ++ [n'] }; and_intros
+      exists { s with queue := s.queue ++ [n'] }; 
+      have Hphi' : φ { lock := i.lock, queue := i.queue ++ [n'] } { queue := s.queue ++ [n'] } := by rw [←i_wf,←s_wf]; apply Hphi
+      and_intros
       · apply star.plus_one; constructor
-      · rw [←i_wf,←s_wf]; apply Hphi
+      · assumption
+      · unfold indistinguishable at *
+        intros e' i' Histep
+        cases Histep with
+        | handle_enq n' a' => constructor; apply star.plus_one; constructor
+        | handle_deq n'' rst' a' =>
+          
     | handle_deq n' rst Hqueue =>
       let Himp2' : ∀ n, imp_step (i_ne n) [Method.deq n'] _ := by
         intros n''; rw [i_wf, Hqueue]; constructor; simp; rfl
@@ -145,7 +254,7 @@ theorem enough :
       have iH'' := iH'; clear iH'
       rcases s with ⟨ queue ⟩
       rcases queue with _ | ⟨ a, b ⟩
-      
+
       constructor; and_intros
       
 
